src/study/Nemonuri.Study.CSharpSyntaxRewriter2.Modifier2/Nemonuri.StratifiedNodes.Nodes.Bijections.ToNode.fst
@@ -1,46 +1,67 @@
 module Nemonuri.StratifiedNodes.Nodes.Bijections.ToNode
 
 module I = Nemonuri.StratifiedNodes.Internals
-module Base = Nemonuri.StratifiedNodes.Nodes.Base
-open Nemonuri.StratifiedNodes.Nodes.Base.Members
+module B = Nemonuri.StratifiedNodes.Nodes.Base
+//open Nemonuri.StratifiedNodes.Nodes.Base.Members
 
 //--- private theory members ---
-private let to_node_impl #t #level (node_internal:I.node_internal t level) : Tot (Base.node t) =
-  Base.SNode level node_internal
+private let to_node_impl #t #level (node_internal:I.node_internal t level) : Tot (B.node t) =
+  B.SNode level node_internal
 
-private let to_node_inverse_impl #t (nd:Base.node t) : Tot (I.node_internal t (get_level nd)) =
-  nd.internal
+private let to_node_inverse_impl #t (node:B.node t) : Tot (I.node_internal t (B.get_level node)) =
+  node.internal
 //---|
 
 //--- propositions ---
 let applying_to_node_inverse_after_to_node_is_identity 
   #t #node_internal_level (node_internal:I.node_internal t node_internal_level) : prop =
-  to_node_inverse_impl (to_node_impl node_internal) == node_internal
+  let result = to_node_inverse_impl (to_node_impl node_internal) in
+  (I.get_level node_internal = node_internal_level) &&
+  (to_node_inverse_impl (to_node_impl node_internal) = node_internal)
 
 let applying_to_node_after_to_node_inverse_is_identity
-  #t (node:Base.node t) : prop =
-  to_node_impl (to_node_inverse_impl node) == node
+  #t (node:B.node t) : prop =
+  to_node_impl (to_node_inverse_impl node) = node
 
 let to_node_is_bijection (t:eqtype) : prop =
   (forall (node_internal_level:pos) (node_internal:I.node_internal t node_internal_level).
     applying_to_node_inverse_after_to_node_is_identity node_internal) /\
-  (forall (node:Base.node t). applying_to_node_after_to_node_inverse_is_identity node)
+  (forall (node:B.node t). applying_to_node_after_to_node_inverse_is_identity node)
+
+let to_node_and_to_node_inverse_are_bijection_pair (t:eqtype) : prop =
+  (forall (node_internal_level:pos) (node_internal:I.node_internal t node_internal_level) (node:B.node t).
+    ((to_node_impl node_internal) = node) <==> 
+    ((B.get_level node = node_internal_level) && (to_node_inverse_impl node = node_internal))
+  )
+
+let to_node_theorem (t:eqtype) : prop =
+  to_node_is_bijection t /\ to_node_and_to_node_inverse_are_bijection_pair t
 //---|
 
 //--- lemma ---
 let lemma_to_node_is_bijection (t:eqtype)
   : Lemma (ensures to_node_is_bijection t) =
   ()
+
+let lemma_to_node_and_to_node_inverse_are_bijection_pair (t:eqtype)
+  : Lemma (ensures to_node_and_to_node_inverse_are_bijection_pair t) =
+  ()
+
+let lemma_to_node_theorem (t:eqtype)
+  : Lemma (ensures to_node_theorem t) =
+  lemma_to_node_is_bijection t;
+  lemma_to_node_and_to_node_inverse_are_bijection_pair t
 //---|
 
 //--- theory members ---
 let to_node #t #level (node_internal:I.node_internal t level)
-  : Pure (Base.node t) True (ensures fun _ -> to_node_is_bijection t) =
-  lemma_to_node_is_bijection t;
+  : Pure (B.node t) True (ensures fun _ -> to_node_theorem t) =
+  lemma_to_node_theorem t;
   to_node_impl node_internal
 
-let to_node_inverse #t (node:Base.node t)
-  : Pure (I.node_internal t (get_level node)) True (ensures fun _ -> to_node_is_bijection t) =
-  lemma_to_node_is_bijection t;
+let to_node_inverse #t (node:B.node t)
+  : Pure (I.node_internal t (B.get_level node)) True 
+    (ensures fun _ -> to_node_theorem t) =
+  lemma_to_node_theorem t;
   to_node_inverse_impl node
 //---|
