src/study/Nemonuri.Study.CSharpSyntaxRewriter2.Modifier2/Nemonuri.StratifiedNodes.Nodes.Bijections.ToNodeList.fst
@@ -1,21 +1,19 @@
 module Nemonuri.StratifiedNodes.Nodes.Bijections.ToNodeList
 
+module L = FStar.List.Tot
 module I = Nemonuri.StratifiedNodes.Internals
-module Base = Nemonuri.StratifiedNodes.Nodes.Base
-module ToNode = Nemonuri.StratifiedNodes.Nodes.Bijections.ToNode
+module B = Nemonuri.StratifiedNodes.Nodes.Base
 open Nemonuri.StratifiedNodes.Nodes.Bijections.ToNode
-open Nemonuri.StratifiedNodes.Nodes.Base.Members
-
 
 //--- private theory members ---
 private let to_node_list_impl #t #max_level 
   (node_list_internal:I.node_list_internal t max_level) 
-  : Tot (Base.node_list t) =
+  : Tot (B.node_list t) =
   I.select node_list_internal (fun ni -> to_node ni)  
 
 private let rec to_node_list_inverse_impl
-  #t (l:Base.node_list t)
-  : Tot (I.node_list_internal t (get_list_level l))
+  #t (l:B.node_list t)
+  : Tot (I.node_list_internal t (B.get_list_level l))
         (decreases l)
   =
   match l with
@@ -26,4 +24,110 @@ private let rec to_node_list_inverse_impl
       I.SCons hd2 tl2
 //---|
 
+//--- propositions ---
+let applying_to_node_list_inverse_after_to_node_list_is_identity 
+  #t #node_list_internal_level
+  (node_list_internal:I.node_list_internal t node_list_internal_level) : prop =
+  let result = to_node_list_inverse_impl (to_node_list_impl node_list_internal) in
+  (I.get_list_level result = node_list_internal_level) &&
+  (result = node_list_internal)
 
+let applying_to_node_list_after_to_node_list_inverse_is_identity 
+  #t (node_list:B.node_list t) : prop =
+  (to_node_list_impl (to_node_list_inverse_impl node_list)) = node_list
+
+let to_node_list_is_bijection (t:eqtype) : prop =
+  (forall (node_list_internal_level:nat) 
+    (node_list_internal:I.node_list_internal t node_list_internal_level).
+    applying_to_node_list_inverse_after_to_node_list_is_identity node_list_internal) /\
+  (forall (node_list:B.node_list t). applying_to_node_list_after_to_node_list_inverse_is_identity node_list)
+
+let to_node_list_and_to_node_list_inverse_are_bijection_pair (t:eqtype) : prop =
+  (forall (node_list_internal_level:nat) 
+    (node_list_internal:I.node_list_internal t node_list_internal_level) 
+    (node_list:B.node_list t).
+    ((to_node_list_impl node_list_internal) = node_list) <==> 
+    ((B.get_list_level node_list = node_list_internal_level) && 
+     (to_node_list_inverse_impl node_list = node_list_internal))
+  )
+
+let length_is_invariant_of_to_node_list 
+  #t #node_list_internal_level
+  (node_list_internal:I.node_list_internal t node_list_internal_level) : prop = 
+  (I.get_length node_list_internal) = (L.length (to_node_list_impl node_list_internal))
+
+let to_node_list_theorem (t:eqtype) : prop =
+  to_node_list_is_bijection t /\
+  to_node_list_and_to_node_list_inverse_are_bijection_pair t
+//---|
+
+//--- lemma ---
+let rec lemma_applying_to_node_list_inverse_after_to_node_list_is_identity
+  #t #node_list_internal_level
+  (node_list_internal:I.node_list_internal t node_list_internal_level)
+  : Lemma (ensures applying_to_node_list_inverse_after_to_node_list_is_identity node_list_internal)
+          (decreases node_list_internal)
+  =
+  match node_list_internal with
+  | I.SNil -> ()
+  | I.SCons hd tl -> lemma_applying_to_node_list_inverse_after_to_node_list_is_identity tl
+
+let rec lemma_applying_to_node_list_after_to_node_list_inverse_is_identity
+  #t (node_list:B.node_list t) 
+  : Lemma (ensures applying_to_node_list_after_to_node_list_inverse_is_identity node_list)
+          (decreases node_list)
+  = 
+  match node_list with
+  | [] -> ()
+  | hd::tl -> (
+      assert ((to_node (to_node_inverse hd)) = hd);
+      lemma_applying_to_node_list_after_to_node_list_inverse_is_identity tl
+    )
+
+let lemma_to_node_list_is_bijection (t:eqtype)
+  : Lemma (ensures to_node_list_is_bijection t)
+  =
+  (introduce forall (node_list_internal_level:nat) 
+    (node_list_internal:I.node_list_internal t node_list_internal_level).
+    applying_to_node_list_inverse_after_to_node_list_is_identity node_list_internal with
+    lemma_applying_to_node_list_inverse_after_to_node_list_is_identity node_list_internal);
+  (introduce forall (node_list:B.node_list t).
+    applying_to_node_list_after_to_node_list_inverse_is_identity node_list with
+    lemma_applying_to_node_list_after_to_node_list_inverse_is_identity node_list)
+
+let lemma_to_node_list_and_to_node_list_inverse_are_bijection_pair (t:eqtype)
+  : Lemma (ensures to_node_list_and_to_node_list_inverse_are_bijection_pair t)
+  =
+  lemma_to_node_list_is_bijection t
+
+let lemma_length_is_invariant_of_to_node_list
+  #t #node_list_internal_level
+  (node_list_internal:I.node_list_internal t node_list_internal_level)
+  : Lemma (ensures length_is_invariant_of_to_node_list node_list_internal)
+  =
+  admit ()
+
+let lemma_to_node_list_theorem (t:eqtype) 
+  : Lemma (ensures to_node_list_theorem t)
+  =
+  lemma_to_node_list_is_bijection t;
+  lemma_to_node_list_and_to_node_list_inverse_are_bijection_pair t
+//---|
+
+//--- theory members ---
+let to_node_list #t #max_level 
+  (node_list_internal:I.node_list_internal t max_level) 
+  : Pure (B.node_list t) True 
+    (ensures fun _ -> to_node_list_theorem t)
+  =
+  lemma_to_node_list_theorem t;
+  to_node_list_impl node_list_internal
+
+let to_node_list_inverse
+  #t (node_list:B.node_list t)
+  : Pure (I.node_list_internal t (B.get_list_level node_list)) True
+    (ensures fun _ -> to_node_list_theorem t)
+  =
+  lemma_to_node_list_theorem t;
+  to_node_list_inverse_impl node_list
+//---|
